a large refactoring of the reification plugin.

src/reify_Core.mli
@@ -1,0 +1,66 @@
+type map_sort =
+    SimpleMap
+  | TypedMap
+  | TypedMapAbs of Term.constr
+type map_type =
+  { table_name : Term.constr
+  ; table_elem_type : Term.constr
+  ; table_elem_ctor : Term.constr
+  ; table_scheme : map_sort
+  }
+
+type use_or_bind =
+    Use
+  | RBind
+  | RSkip
+
+type table_name = Term.constr
+
+type command =
+    Rec        of int
+  | Fix        of command
+  | Or         of command * command
+  | Fail
+  | Call       of Term.constr
+  | Map        of Term.constr * command
+  | App        of command * command * Term.constr
+  | Abs        of command * command * Term.constr
+  | Var        of Term.constr
+  | PiMeta     of Term.constr * command
+  | Patterns   of Term.constr
+  | Pattern    of rule list
+  | Table      of table_name
+  | TypedTable of table_name * command (** To parse the type *)
+
+and rpattern =
+    RIgnore
+  | RHasType of Term.constr * rpattern
+  | RConst
+  | RGet   of int * rpattern
+  | RApp   of rpattern * rpattern
+  | RPi    of rpattern * use_or_bind * rpattern
+  | RLam   of rpattern * rpattern
+  | RImpl  of rpattern * rpattern
+  | RExact of Term.constr
+
+and action =
+    Func of command
+  | Id
+
+and template =
+    Bind of action * template
+  | Return of Term.constr
+
+(** [rule]s implement the pattern feature **)
+and rule =
+  { rule_pattern  : rpattern
+  ; rule_template : template
+  }
+
+exception ParseFailure of Term.constr * string
+
+val parse_command : Environ.env -> Evd.evar_map -> Term.constr -> command
+
+val parse_pattern : Environ.env -> Evd.evar_map -> Term.constr -> Term.constr -> rule
+
+val parse_tables : Term.constr -> map_type list
