src/reify_Monad.ml
@@ -1,0 +1,77 @@
+module Cmap = Map.Make
+    (struct
+      type t = Term.constr
+      let compare = Term.constr_ord
+    end)
+
+module IntMap = Map.Make
+    (struct
+      type t = int
+      let compare = Int.compare
+    end)
+
+exception ReificationFailure of (Term.constr Lazy.t)
+
+type lazy_term =
+  | Term of Term.constr
+  | App of Term.constr * Term.constr array * int
+
+let get_term (trm : lazy_term) =
+  match trm with
+    Term trm -> trm
+  | App (trm,args,from) ->
+    if from = -1 then trm
+    else if from = Array.length args then
+      Term.mkApp (trm, args)
+    else Term.mkApp (trm, Array.sub args 0 (from+1))
+
+type 'a environment =
+  { mappings : 'a Cmap.t
+  ; next     : int
+  }
+
+type reify_env =
+  { env : Environ.env
+  ; evm : Evd.evar_map
+  ; bindings : Reify_Core.use_or_bind list
+  ; typed_tables : (int * Term.constr) environment Cmap.t ref
+  }
+
+(** [reifier]s are the actual functions that get run **)
+type 'a reifier =
+  reify_env -> 'a
+
+let reifier_bind (c : 'a reifier) (k : 'a -> 'b reifier) : 'b reifier =
+  fun gl ->
+    k (c gl) gl
+
+let reifier_fmap (f : 'a -> 'b) (c : 'a reifier) : 'b reifier =
+  fun gl -> f (c gl)
+
+let reifier_fail (t : Term.constr) : 'a reifier =
+  fun gl -> raise (ReificationFailure (lazy t))
+
+let reifier_fail_lazy (t : lazy_term) : 'a reifier =
+  fun gl -> raise (ReificationFailure (lazy (get_term t)))
+
+let reifier_try (c : 'a reifier) (x : 'a reifier) : 'a reifier =
+  fun gl ->
+    try c gl
+    with ReificationFailure _ -> x gl
+
+let reifier_ret (value : 'a) : 'a reifier =
+  fun _ -> value
+let reifier_get_env : reify_env reifier =
+  fun e -> e
+
+let reifier_local (f : reify_env -> reify_env) (c : 'a reifier) : 'a reifier =
+  fun gl -> c (f gl)
+
+let reifier_under_binder ?name:(name=Names.Anonymous)
+    (b : Reify_Core.use_or_bind) (t : Term.constr) (c : 'a reifier)
+  : 'a reifier =
+  fun gl -> c { gl with
+                bindings = b :: gl.bindings
+              ; env = Environ.push_rel (name, None, t) gl.env }
+
+let reifier_run (c : 'a reifier) (gl : reify_env) = c gl
