theories/Reify/Reify.v
@@ -5,3 +5,6 @@ Require MirrorCore.Lemma.
 Declare ML Module "reify_Lambda_plugin".
 
 Export MirrorCore.Reify.Patterns.
+
+Class Reify (T : Type) : Type :=
+  reify_scheme : Command T.
